examples/MOD.v
@@ -1,63 +1,134 @@
-Require Import Common Core. 
+Require Import Common. 
+Require Core TaggedUnions. 
 
-Section t. 
-  Variable n : nat. 
-  Notation NUM := (Tlift (Tint n)). 
-  Notation VAL := (Tlift (Tbool)) (only parsing). 
-  Definition Phi : state := (Treg VAL :: Treg NUM  :: Treg NUM :: nil)%list. 
+Module Ex1. 
+  Import TaggedUnions. 
+  
+  Section t. 
+    Variable n : nat. 
+    
+    Definition T : type := 
+      Tunion ([Int n; Ttuple [Int n; Int n]])%list.
+        
+    Notation MOD := (var_S var_0). 
+    Notation VAL := var_0. 
 
-  Notation c := (var_0 : var Phi (Treg VAL)).
-  Notation r1 := (var_S (var_0) : var Phi (Treg NUM)).  
-  Notation r2 := (var_S (var_S (var_0)) : var Phi (Treg NUM)).  
+    Definition Phi : state := (Treg T :: nil)%list. 
+    
+    Notation R := (var_0 : var Phi (Treg T)). 
+    Notation "^ X " := (Econstr _ _ _ X) (at level 1, no associativity). 
+    Definition iterate : Action Phi Unit. intros V.
+    refine (DO R' <- read [: R ]; 
+            (MATCH (!R') IN T WITH MOD OF  A , B ==>  
+                  (
+                    WHEN (!B <= !A);
+                    DO _ <- (write [: R <- ^ MOD [< !A - !B ; !B >]]);
+                    Return (#Ctt)
+                  )
+           )). 
+    Defined. 
+    
+    Definition done : Action Phi Unit. intros V. 
+    refine (DO R' <- read [: R];
+            (MATCH (!R') IN T WITH MOD OF A, B ==> 
+                   (
+                     WHEN (!A < !B);
+                     DO _ <- (write [: R <- ^ VAL (!A) ]);
+                     Return (#Ctt)
+                   )
+           )). 
+    Defined. 
+    
+    Definition This : TRS := mk_TRS Phi (iterate :: done :: nil)%list. 
+    
+    Inductive Ty : Type :=
+    | RET : Word.T n -> Ty
+    | ST : Word.T n -> Word.T n -> Ty. 
+    
+    
+    Definition start (x : Ty) : eval_state Phi :=
+      match x with 
+        | RET a => inl a
+        | ST a b => inr (inl (a,b))
+      end.
 
-  Definition iterate : Action Phi Unit. intros V.
-  refine (DO X <- read [: c]; 
-          WHEN ( !X); 
-          DO A <- read [: r1]; 
-          DO B <- read [: r2];
-          WHEN (!B <= !A); 
-          DO _ <- (write [: r1 <- (!A - !B)]);  
-          (* DO _ <- (write [: r2 <- (!B)]);   *)
-          RETURN #Ctt
-         ). 
-  Defined. 
+    Definition finish (x : eval_state Phi) : Ty :=
+      match x with
+        | inl t => RET t
+        | inr (inl p) => ST (fst p) (snd p)
+        | inr (inr f) => False_rec Ty f
+      end. 
+    
+    Definition st0 x y := start (ST (Word.repr n x) (Word.repr n y)). 
+    
+    Definition finish' x := match x with None => None | Some x => Some (finish x) end. 
+  End t. 
   
-  Definition done : Action Phi Unit. intros V. 
-  refine (DO X <- read [: c]; 
-          WHEN (!X); 
-          DO A <- read [: r1]; 
-          DO B <- read [: r2];
-          WHEN (!A < !B); 
-          DO _ <- (write [: c <- #b false]);  
-          (* DO _ <- (write [: r1 <- !A ]);   *)
-          RETURN #Ctt
-         ). 
-  Defined. 
-  
-  Definition T : TRS := mk_TRS Phi (iterate :: done :: nil)%list. 
-  
-  Inductive Ty : Type :=
-  | RET : Word.T n -> Ty
-  | ST : Word.T n -> Word.T n -> Ty. 
-  
-  Definition start (x : Ty) : eval_state Phi :=
-    match x with 
-      | RET a => (false, (a, (a, tt)))
-      | ST a b => (true, (a, (b, tt)))
-    end.
-  
-  Definition finish (x : eval_state Phi) : Ty :=
-    match x with 
-      | (c,(a,(b,_))) => 
-          match c with 
-            | true => ST a b
-            | false => RET a
-          end
-    end. 
-  
-  Definition st0 x y := start (ST (Word.repr n x) (Word.repr n y)). 
-  
-  Definition finish' x := match x with None => None | Some x => Some (finish x) end. 
-End t. 
+  Eval compute in finish' 16 (run_unfair (This 16) 10 (st0 16 17 3)). 
+End Ex1. 
 
-Eval compute in finish' 16 (run_unfair (T 16) 10 (st0 16 17 3)). 
+Module  Ex2. 
+  Import Core. 
+  
+  Section t. 
+    Variable n : nat. 
+    Notation NUM := (Tlift (Tint n)). 
+    Notation VAL := (Tlift (Tbool)) (only parsing). 
+    Definition Phi : state := (Treg VAL :: Treg NUM  :: Treg NUM :: nil)%list. 
+    
+    Notation c := (var_0 : var Phi (Treg VAL)).
+    Notation r1 := (var_S (var_0) : var Phi (Treg NUM)).  
+    Notation r2 := (var_S (var_S (var_0)) : var Phi (Treg NUM)).  
+
+    Definition iterate : Action Phi Unit. intros V.
+    refine (DO X <- read [: c]; 
+            WHEN ( !X); 
+            DO A <- read [: r1]; 
+            DO B <- read [: r2];
+            WHEN (!B <= !A); 
+            DO _ <- (write [: r1 <- (!A - !B)]);  
+            (* DO _ <- (write [: r2 <- (!B)]);   *)
+            RETURN #Ctt
+           ). 
+    Defined. 
+    
+    Definition done : Action Phi Unit. intros V. 
+    refine (DO X <- read [: c]; 
+            WHEN (!X); 
+            DO A <- read [: r1]; 
+            DO B <- read [: r2];
+            WHEN (!A < !B); 
+            DO _ <- (write [: c <- #b false]);  
+            (* DO _ <- (write [: r1 <- !A ]);   *)
+            RETURN #Ctt
+           ). 
+    Defined. 
+    
+    Definition T : TRS := mk_TRS Phi (iterate :: done :: nil)%list. 
+    
+    Inductive Ty : Type :=
+    | RET : Word.T n -> Ty
+    | ST : Word.T n -> Word.T n -> Ty. 
+    
+    Definition start (x : Ty) : eval_state Phi :=
+      match x with 
+        | RET a => (false, (a, (a, tt)))
+        | ST a b => (true, (a, (b, tt)))
+      end.
+    
+    Definition finish (x : eval_state Phi) : Ty :=
+      match x with 
+        | (c,(a,(b,_))) => 
+            match c with 
+              | true => ST a b
+              | false => RET a
+            end
+      end. 
+    
+    Definition st0 x y := start (ST (Word.repr n x) (Word.repr n y)). 
+    
+    Definition finish' x := match x with None => None | Some x => Some (finish x) end. 
+  End t. 
+  
+  Eval compute in finish' 16 (run_unfair (T 16) 10 (st0 16 17 3)). 
+End Ex2. 
